Begin diagrams combinators

theories/Diagrams.v
@@ -1,11 +1,96 @@
 
 From HoTT Require Import Basics.
 From HoTT Require Import Categories.
-Require Import CommutativeDiagrams.Loader.
+From HoTT Require Import Spaces.Finite.
+From HoTT Require Import Spaces.Nat.
+From HoTT Require Import Spaces.List.
 
-HelloWorld.
+Section Diagrams.
+  Variable C : PreCategory.
+  Variable Node Vertex Face : Type.
+  Variable Index : Type.
+  Variable Hid : DecidablePaths Index.
 
-Lemma test : True.
-Proof.
-  hello. exact I.
-Qed.
+  Record NodeData :=
+    mkNodeData
+      { node_object : object C
+      ; node_name   : option Index
+      }.
+  Record VertexData {nodes : Node -> NodeData} :=
+    mkVertexData
+      { vertex_src : Node
+      ; vertex_dst : Node
+      ; vertex_mph : morphism C (node_object (nodes vertex_src)) (node_object (nodes vertex_dst))
+      ; vertex_name : option Index
+      }.
+  Arguments VertexData nodes : clear implicits.
+  Definition eqToIso {a b : object C} (p : a = b) : morphism C a b :=
+    paths_ind a (fun b _ => morphism C a b) 1%morphism b p.
+  Definition conjugate {a b c d : object C} (f : morphism C b c) (p1 : a = b) (p2 : d = c) :
+    morphism C a d :=
+    eqToIso p2^ o f o (eqToIso p1).
+  Record FaceData {nodes : Node -> NodeData} {vertices : Vertex -> VertexData nodes} :=
+    mkFaceData
+      { face_src : Vertex
+      ; face_dst : Vertex
+      ; face_src_eq : node_object (nodes (vertex_src (vertices face_src)))
+                      = node_object (nodes (vertex_src (vertices face_dst)))
+      ; face_dst_eq : node_object (nodes (vertex_dst (vertices face_src)))
+                      = node_object (nodes (vertex_dst (vertices face_dst)))
+      ; face : vertex_mph (vertices face_src)
+               = conjugate (vertex_mph (vertices face_dst)) face_src_eq face_dst_eq
+      ; face_name : option Index
+      }.
+  Arguments FaceData nodes vertices : clear implicits.
+  Record Diagram :=
+    mkDiagram
+      { gr_node : Node -> NodeData
+      ; gr_vertex : Vertex -> VertexData gr_node
+      ; gr_face : Face -> FaceData gr_node gr_vertex
+      }.
+End Diagrams.
+
+Section Combinators.
+  Context {C : PreCategory}.
+  Context {Node1 Node2 Vertex1 Vertex2 Face1 Face2 : Type}.
+  Context {Index : Type}.
+  Context {Hid : DecidablePaths Index}.
+
+  Variable d1 : Diagram C Node1 Vertex1 Face1 Index.
+  Variable d2 : Diagram C Node2 Vertex2 Face2 Index.
+
+  Ltac empty_ind := apply Empty_ind; assumption.
+
+  Definition emptyD : Diagram C Empty Empty Empty Index.
+  Proof. srapply mkDiagram; intros; empty_ind. Defined.
+
+  Definition singletonD (x : object C) (label : option Index) :
+    Diagram C Unit Empty Empty Index.
+  Proof.
+    srapply mkDiagram; intros; [ | empty_ind | empty_ind ].
+    srapply mkNodeData; [ exact x | exact label ].
+  Defined.
+
+  Definition mkSimpleNodeData : object C -> NodeData C Index :=
+    fun x => mkNodeData C Index x None.
+
+  Definition arrowD {s d : object C} (m : morphism C s d) (label : option Index) :
+    Diagram C (Fin 2) Unit Empty Index.
+  Proof.
+    srapply mkDiagram; [ | | empty_ind ].
+    - intro x. destruct x; srapply mkSimpleNodeData; [ exact d | exact s ].
+    - intros _. srapply mkVertexData; [ exact (inr tt) | exact (inl (inr tt)) | exact m | exact label ].
+  Defined.
+
+  Definition faceD {s d : object C} {m1 m2 : morphism C s d} (f : m1 = m2) (label : option Index) :
+    Diagram C (Fin 2) (Fin 2) Unit Index.
+  Proof.
+    srapply mkDiagram.
+    - intro x. destruct x; srapply mkSimpleNodeData; [ exact d | exact s ].
+    - intro x. srapply mkVertexData; [ exact (inr tt) | exact (inl (inr tt)) | | exact None ].
+      destruct x; [ exact m2 | exact m1 ].
+    - intros _. srapply mkFaceData; [ exact (inr tt) | exact (inl (inr tt)) | exact 1 | exact 1 | | exact label ].
+      unfold conjugate. simpl. rewrite left_identity. rewrite right_identity. exact f.
+  Defined.
+
+End Combinators.
